configScript.sml
@@ -1,0 +1,31 @@
+
+open HolKernel Parse boolLib bossLib term_tactic;
+open arithmeticTheory integerTheory stringTheory optionTheory;
+
+val _ = new_theory "config";
+
+(*
+ * A basic configuration that supports integers and strings. This configuration
+ * is hardcoded into the types defined in [{exp,value,pure_lang}Script.sml].
+ *)
+
+Datatype:
+  lit = Int int
+      | Str string
+End
+
+Datatype:
+  atom = Add | Concat | Length
+End
+
+Definition atom_op_def:
+  atom_op op args =
+    case (op, args) of
+      (Add, [Int x; Int y]) => SOME (Int (x + y))
+    | (Concat, [Str s; Str t]) => SOME (Str (STRCAT s t))
+    | (Length, [Str s]) => SOME (Int &(STRLEN s))
+    | _ => NONE
+End
+
+val _ = export_theory ();
+
